assembler/RealAsm.v
@@ -1,0 +1,81 @@
+Require Import Smallstep.
+Require Import Machregs.
+Require Import Asm.
+Require Import Integers.
+Require Import Floats.
+Require Import List.
+Require Import ZArith.
+Require Import Memtype.
+Require Import Memory.
+Require Import Archi.
+Require Import Coqlib.
+Require Import AST.
+Require Import Globalenvs.
+Require Import Events.
+Require Import Values.
+Require Import Conventions1.
+Require Import RealAsmArchi.
+
+Section INSTRSIZE.
+Variable instr_size : instruction -> Z.
+
+Inductive initial_state (p: Asm.program): state -> Prop :=
+  | initial_state_intro: forall m0 m' rs0,
+      Genv.init_mem p = Some m0 ->
+      initial_stack_regset p m0 m' rs0 ->      
+      initial_state p (State rs0 m').
+
+Definition semantics prog :=
+  Semantics (RealAsmArchi.step instr_size) (initial_state prog) final_state (Genv.globalenv prog).
+
+Section RECEPTIVEDET.
+
+  Theorem real_asm_single_events p:
+    single_events (semantics p).
+  Proof.
+    red. simpl. intros s t s' STEP.
+    inv STEP; simpl. lia.
+    eapply external_call_trace_length; eauto.
+    (* eapply external_call_trace_length; eauto. *)
+  Qed.
+
+  Theorem real_asm_receptive p:
+    receptive (semantics p).
+  Proof.
+    split.
+    - simpl. intros s t1 s1 t2 STEP MT.
+      inv STEP.
+      inv MT. eexists. eapply exec_step_internal; eauto.
+      edestruct external_call_receptive as (vres2 & m2 & EC2); eauto.
+      (* eexists. eapply exec_step_builtin; eauto. *)
+      (* edestruct external_call_receptive as (vres2 & m2 & EC2); eauto. *)
+      eexists. eapply exec_step_external; eauto.
+    - eapply real_asm_single_events; eauto.
+  Qed.
+
+  Ltac rewrite_hyps :=
+  repeat
+    match goal with
+      H1 : ?a = _, H2: ?a = _ |- _ => rewrite H1 in H2; inv H2
+    end.
+
+  Theorem real_asm_determinate p :
+    determinate (semantics p).
+  Proof.
+    split.
+    - simpl; intros s t1 s1 t2 s2 STEP1 STEP2.
+      eapply semantics_determinate_step;eauto.
+    - apply real_asm_single_events.
+    - simpl. intros s1 s2 IS1 IS2; inv IS1; inv IS2. rewrite_hyps.
+      inv H0; inv H2. rewrite_hyps. unfold rs0, rs2, ge, ge0 in *. rewrite_hyps. congruence.
+    - simpl. intros s r FS.
+      red. intros t s' STEP.
+      inv FS.
+      unfold Vnullptr in *. destruct Archi.ptr64;inv STEP;rewrite_hyps. 
+    - simpl. intros s r1 r2 FS1 FS2.
+      inv FS1; inv FS2. congruence.
+  Qed.
+
+End RECEPTIVEDET.
+
+End INSTRSIZE.
