x86/RealAsmArchi.v
@@ -1,0 +1,141 @@
+Require Import Smallstep.
+Require Import Machregs.
+Require Import Asm.
+Require Import Integers.
+Require Import Floats.
+Require Import List.
+Require Import ZArith.
+Require Import Memtype.
+Require Import Memory.
+Require Import Archi.
+Require Import Coqlib.
+Require Import AST.
+Require Import Globalenvs.
+Require Import Events.
+Require Import Values.
+Require Import Conventions1.
+
+Definition stkblock := Stack None nil 1.
+
+(** * Operational Semantics with instr_size *)
+Section INSTRSIZE.
+Variable instr_size : instruction -> Z.
+
+Section WITHGE.
+  Variable ge : Genv.t Asm.fundef unit.
+
+  Definition exec_instr f i rs (m: mem) :=
+    let isz := Ptrofs.repr (instr_size i) in
+    match i with
+    | Pallocframe sz ofs_ra ofs_link =>
+      let aligned_sz := (* align sz 8 *) sz in
+      let psp := (Val.offset_ptr (rs#RSP) (Ptrofs.repr (size_chunk Mptr))) in (* parent stack pointer *)
+      let sp := Val.offset_ptr (rs#RSP) (Ptrofs.neg (Ptrofs.sub (Ptrofs.repr aligned_sz) (Ptrofs.repr (size_chunk Mptr)))) in
+      match Mem.storev Mptr m (Val.offset_ptr sp ofs_link) psp with
+        |None => Stuck
+        |Some m1 =>
+      Next (nextinstr_nf isz (rs #RAX <- (Val.offset_ptr (rs RSP) (Ptrofs.repr (size_chunk Mptr))) #RSP <- sp)) m1
+      end
+    | Pfreeframe sz ofs_ra ofs_link =>
+      let sp := Val.offset_ptr (rs RSP) (Ptrofs.sub (Ptrofs.repr (*(align sz 8)*) sz) (Ptrofs.repr (size_chunk Mptr))) in
+      Next (nextinstr isz (rs#RSP <- sp)) m
+    | Pcall_s i sg =>
+      let sp := Val.offset_ptr (rs RSP) (Ptrofs.neg (Ptrofs.repr (size_chunk Mptr))) in
+      match Mem.storev Mptr m sp (Val.offset_ptr rs#PC isz) with
+        |None => Stuck
+        |Some m1 =>
+        Next (rs#RA <- (Val.offset_ptr rs#PC isz)
+                #PC <- (Genv.symbol_address ge i Ptrofs.zero)
+                #RSP <- sp) m1
+      end
+    |Pcall_r r sg =>
+      let sp := Val.offset_ptr (rs RSP) (Ptrofs.neg (Ptrofs.repr (size_chunk Mptr))) in
+      match Mem.storev Mptr m sp (Val.offset_ptr rs#PC isz) with
+        |None => Stuck
+        |Some m1 =>
+        Next (rs#RA <- (Val.offset_ptr rs#PC isz)
+                #PC <- (rs r)
+                #RSP <- sp) m1
+      end
+    | Pret =>
+      match loadvv Mptr m rs#RSP with
+      | None => Stuck
+      | Some ra =>
+        let sp := Val.offset_ptr (rs RSP) (Ptrofs.repr (size_chunk Mptr)) in
+        Next (rs #RSP <- sp
+                 #PC <- ra
+                 #RA <- Vundef) m
+      end
+    | _ => exec_instr instr_size ge f i rs m
+    end.
+
+  Inductive step  : state -> trace -> state -> Prop :=
+  | exec_step_internal:
+      forall b ofs f i rs m rs' m',
+        rs PC = Vptr b ofs ->
+        Genv.find_funct_ptr ge b = Some (Internal f) ->
+        find_instr instr_size (Ptrofs.unsigned ofs) (fn_code f) = Some i ->
+        exec_instr f i rs m = Next rs' m' ->
+        step (State rs m) E0 (State rs' m')
+  | exec_step_external:
+      forall b ef args res rs m t rs' m',
+      rs PC = Vptr b Ptrofs.zero ->
+      Genv.find_funct_ptr ge b = Some (External ef) ->
+      extcall_arguments
+        (rs # RSP <- (Val.offset_ptr (rs RSP) (Ptrofs.repr (size_chunk Mptr)))) m (ef_sig ef) args ->
+        forall (SP_TYPE: Val.has_type (rs RSP) Tptr)
+          ra (LOADRA: Mem.loadv Mptr m (rs RSP) = Some ra)
+          (SP_NOT_VUNDEF: rs RSP <> Vundef)
+          (RA_NOT_VUNDEF: ra <> Vundef),
+      external_call ef ge args m t res m' ->
+      rs' = (set_pair (loc_external_result (ef_sig ef))
+                      res (undef_caller_save_regs rs))
+              #PC <- ra
+              #RA <- Vundef
+              #RSP <- (Val.offset_ptr (rs RSP) (Ptrofs.repr (size_chunk Mptr)))
+      ->
+      step (State rs m) t (State rs' m').
+
+End WITHGE.
+
+Inductive initial_stack_regset (p: Asm.program) (m0: mem) : mem -> regset -> Prop :=
+| initial_state_archi_archi: forall m1 m2 stk bmain,
+    Mem.alloc m0 0 (max_stacksize + (align (size_chunk Mptr)8)) = (m1, stk) ->
+    Mem.storev Mptr m1 (Vptr stk (Ptrofs.repr (max_stacksize + align (size_chunk Mptr) 8 - size_chunk Mptr))) Vnullptr = Some m2 ->
+    let ge := Genv.globalenv p in
+    Genv.find_symbol ge p.(prog_main) = Some bmain ->
+    let rs0 :=
+      (Pregmap.init Vundef)
+        # PC <- (Vptr bmain Ptrofs.zero)
+        # RA <- Vnullptr
+        # RSP <- (Val.offset_ptr
+                   (Vptr stkblock (Ptrofs.repr (max_stacksize + align (size_chunk Mptr) 8)))
+                   (Ptrofs.neg (Ptrofs.repr (size_chunk Mptr)))) in
+    initial_stack_regset p m0 m2 rs0.
+
+  Ltac rewrite_hyps :=
+  repeat
+    match goal with
+      H1 : ?a = _, H2: ?a = _ |- _ => rewrite H1 in H2; inv H2
+    end.
+
+  Ltac Equalities :=
+  match goal with
+  | [ H1: ?a = ?b, H2: ?a = ?c |- _ ] =>
+      rewrite H1 in H2; inv H2; Equalities
+  | _ => idtac
+  end.
+  
+Lemma semantics_determinate_step : forall p s s1 s2 t1 t2,
+  step (Genv.globalenv p) s t1 s1 ->
+  step (Genv.globalenv p) s t2 s2 -> match_traces (Genv.globalenv p) t1 t2 /\ (t1 = t2 -> s1 = s2).
+Proof.
+  intros.
+  inv H; inv H0; Equalities.
+  split. constructor.  auto.
+  assert (args0 = args) by (eapply extcall_arguments_determ; eauto). subst args0.
+  exploit external_call_determ. eexact H4. eexact H9. intros [A B].
+  split. auto. intros. destruct B; auto. subst. auto.
+Qed.
+
+End INSTRSIZE.
